concurrency/verif_bst_conc_cglock2.v
@@ -1,0 +1,596 @@
+Require Import VST.progs.conclib.
+Require Import VST.floyd.proofauto.
+Require Import VST.floyd.library.
+Require Import bst.bst_conc_cglock.
+Require Import VST.atomics.general_locks.
+Require Import Coq.Sets.Ensembles.
+Require Import Coq.micromega.Lia.
+
+Instance CompSpecs : compspecs. make_compspecs prog. Defined.
+Definition Vprog : varspecs. mk_varspecs prog. Defined.
+
+Definition t_struct_tree := Tstruct _tree noattr.
+Definition t_struct_tree_t := Tstruct _tree_t noattr.
+
+Section TREES.
+  Context { V : Type }.
+  Variable default: V.
+
+  Definition key := Z.
+
+  Inductive tree : Type :=
+  | E : tree
+  | T: tree -> key -> V -> tree -> tree.
+
+  Inductive In (k : key) : tree -> Prop :=
+  | InRoot l r x v:  (k = x) -> In k (T l x v r )
+  | InLeft l r x v': In k l -> In k (T l x v' r)
+  | InRight l r x v': In k r -> In k (T l x v' r).
+
+  Definition lt (t: tree) (k: key) := forall x : key, In x t -> k < x .
+  Definition gt (t: tree) (k: key) := forall x : key, In x t -> k > x .
+
+  Inductive sorted_tree : tree -> Prop :=
+  | Sorted_Empty : sorted_tree E
+  | Sorted_Tree x v l r : sorted_tree l -> sorted_tree r ->
+                          gt l x -> lt r x -> sorted_tree (T l x v r ).
+
+  Definition empty_tree : tree := E.
+
+  Fixpoint lookup (x: key) (t : tree) : V :=
+    match t with
+    | E => default
+    | T tl k v tr => if x <? k then lookup x tl
+                     else if k <? x then lookup x tr
+                          else v
+    end.
+
+  Fixpoint insert (x: key) (v: V) (s: tree) : tree :=
+    match s with
+    | E => T E x v E
+    | T a y v' b => if  x <? y then T (insert x v a) y v' b
+                    else if y <? x then T a y v' (insert x v b)
+                         else T a x v b
+    end.
+
+  Fixpoint pushdown_left (a: tree) (bc: tree) : tree :=
+    match bc with
+    | E => a
+    | T b y vy c => T (pushdown_left a b) y vy c
+    end.
+
+  Fixpoint delete (x: key) (s: tree) : tree :=
+    match s with
+    | E => E
+    | T a y v' b => if  x <? y then T (delete x a) y v' b
+                    else if y <? x then T a y v' (delete x b)
+                         else pushdown_left a b
+    end.
+
+  Lemma pushdown_left_In: forall (t1 t2: tree) (x: key),
+      In x (pushdown_left t1 t2) -> In x t1 \/ In x t2.
+  Proof.
+    intros. revert t2 H. induction t2; intros; simpl in *; auto. inv H.
+    - right. now apply InRoot.
+    - apply IHt2_1 in H1. destruct H1; [left | right]; auto. now apply InLeft.
+    - right. now apply InRight.
+  Qed.
+
+  Lemma delete_In: forall (x: key) (t: tree) (y: key), In y (delete x t) -> In y t.
+  Proof.
+    intros. revert t H. induction t; intros; simpl in *; auto. destruct (x <? k).
+    - inv H; try ((now apply InLeft) || (now apply InRoot) || (now apply InRight)).
+      apply IHt1 in H1. now apply InLeft.
+    - destruct (k <? x).
+      + inv H; try ((now apply InLeft) || (now apply InRoot) || (now apply InRight)).
+        apply IHt2 in H1. now apply InRight.
+      + apply pushdown_left_In in H. destruct H; [apply InLeft | apply InRight]; easy.
+  Qed.
+
+  Lemma pushdown_left_sorted: forall (t1 t2: tree),
+      sorted_tree t1 -> sorted_tree t2 -> (forall x y, In x t1 -> In y t2 -> x < y) ->
+      sorted_tree (pushdown_left t1 t2).
+  Proof.
+    intros. revert t2 H0 H1. induction t2; intros; simpl in H0 |-* ; auto.
+    inv H0. constructor; auto.
+    - apply IHt2_1; auto. intros. apply H1; auto. now apply InLeft.
+    - intros z ?. apply pushdown_left_In in H0. destruct H0.
+      + apply Z.lt_gt, H1; auto. now apply InRoot.
+      + now specialize (H8 _ H0).
+  Qed.
+
+  Lemma delete_sorted: forall (x: key) (t: tree),
+      sorted_tree t -> sorted_tree (delete x t).
+  Proof.
+    intros. revert t H. induction t; intros; simpl; auto. inv H.
+    destruct (x <? k) eqn: ?.
+    - apply Z.ltb_lt in Heqb. constructor; auto. intros y ?.
+      apply delete_In in H. now apply H6.
+    - apply Z.ltb_ge in Heqb. destruct (k <? x) eqn: ?.
+      + apply Z.ltb_lt in Heqb0. constructor; auto. intros y ?.
+        apply delete_In in H. now apply H7.
+      + apply pushdown_left_sorted; auto. intros y z ? ?.
+        apply H6 in H. apply H7 in H0. lia.
+  Qed.
+
+  Lemma value_in_tree: forall x v k (t: tree),
+      In k (insert x v t ) -> (x = k) \/ In k t.
+  Proof.
+    intros. induction t; simpl in H. 1: inversion H; subst; auto.
+    destruct (x <? k0) eqn: Heqn.
+    - inversion H; subst.
+      + right. apply InRoot. auto.
+      + specialize (IHt1 H1). destruct IHt1. left. auto. right. apply InLeft. auto.
+      + right. apply InRight. auto.
+    - destruct (k0 <? x) eqn: Heqn'.
+      + inversion H; subst.
+        * right. apply InRoot. auto.
+        * right. apply InLeft. auto.
+        * specialize (IHt2 H1). destruct IHt2. left. auto. right. apply InRight. auto.
+      + assert (k0 = x).
+        { apply Z.ltb_nlt in Heqn'. apply Z.ltb_nlt in Heqn. lia. }
+        subst. right. inversion H; subst.
+        * apply InRoot. auto.
+        * apply InLeft. auto.
+        * apply InRight. auto.
+  Qed.
+
+  Lemma insert_sorted : forall x v (t: tree),
+      sorted_tree t -> sorted_tree (insert x v t).
+  Proof.
+    intros. induction t.
+    - simpl. apply Sorted_Tree; auto; [unfold gt | unfold lt]; intros; easy.
+    - simpl. destruct (x <? k)  eqn: Heqn.
+      + constructor.
+        * apply IHt1. inversion H; auto.
+        * inversion H; auto.
+        * unfold gt. intros. apply value_in_tree in H0. destruct H0. subst.
+          apply Z.ltb_lt in Heqn. lia.  inversion H;subst. auto.
+        * unfold lt. intros. inversion H; subst. auto.
+      + destruct (k <? x) eqn: Heqn'.
+        * apply Sorted_Tree.
+          -- inversion H; subst. auto.
+          -- apply IHt2. inversion H. auto.
+          -- unfold gt. intros. inversion H; subst. auto.
+          -- unfold lt. intros. apply value_in_tree in H0. destruct H0.
+             ++ subst. apply Z.ltb_lt in Heqn'. lia.
+             ++ inversion H; subst. auto.
+        * assert (k = x).
+          {apply Z.ltb_nlt in Heqn'. apply Z.ltb_nlt in Heqn. lia. }
+          subst. apply Sorted_Tree; inversion H; subst; auto.
+  Qed.
+
+End TREES.
+
+Fixpoint tree_rep (t: @tree val) (p: val): mpred :=
+ match t with
+ | E => !!(p=nullval) && emp
+ | T a x v b => !! (Int.min_signed <= x <= Int.max_signed /\ tc_val (tptr Tvoid) v) &&
+   EX pa:val, EX pb:val,
+                    malloc_token Ews t_struct_tree p *
+                    data_at Ews t_struct_tree (Vint (Int.repr x),(v,(pa,pb))) p *
+                    tree_rep a pa * tree_rep b pb
+ end.
+
+Instance tree_ghost: Ghost := discrete_PCM (@tree val).
+
+Notation tree_info := (@G tree_ghost).
+
+Definition treebox_rep (t: @tree val) (b: val) :=
+  EX p: val, data_at Ews (tptr t_struct_tree) p b * tree_rep t p.
+
+Definition node_lock_inv g lock np :=
+  (EX tr, my_half g Tsh tr *
+          treebox_rep tr (field_address t_struct_tree_t [StructField _t] np)) *
+  malloc_token Ews tlock lock * malloc_token Ews t_struct_tree_t np.
+
+Definition nodebox_rep (g : gname)
+           (sh : share) (lock : val) (nb: val) :=
+  EX np: val,
+     data_at sh (tptr t_struct_tree_t) np nb *
+     field_at sh t_struct_tree_t [StructField _lock] lock np *
+     lock_inv sh lock (node_lock_inv g lock np).
+
+Definition surely_malloc_spec :=
+  DECLARE _surely_malloc
+  WITH t:type, gv: globals
+  PRE [ _n OF tuint ]
+    PROP (0 <= sizeof t <= Int.max_unsigned;
+          complete_legal_cosu_type t = true;
+          natural_aligned natural_alignment t = true)
+    LOCAL (temp _n (Vint (Int.repr (sizeof t))); gvars gv)
+    SEP (mem_mgr gv)
+  POST [ tptr tvoid ] EX p:_,
+    PROP ()
+    LOCAL (temp ret_temp p)
+    SEP (mem_mgr gv; malloc_token Ews t p * data_at_ Ews t p).
+
+Program Definition lookup_spec :=
+  DECLARE _lookup
+  ATOMIC TYPE (rmaps.ConstType (val * share * val * Z * globals * gname))
+  OBJ BST INVS base.empty base.top
+  WITH b:_, sh:_, lock:_, x:_, gv:_, g:_
+  PRE [_t OF (tptr (tptr t_struct_tree_t)), _x OF tint]
+   PROP (readable_share sh;
+        Int.min_signed <= x <= Int.max_signed; is_pointer_or_null lock)
+   LOCAL (temp _t b; temp _x (Vint (Int.repr x)); gvars gv)
+   SEP (mem_mgr gv; nodebox_rep g sh lock b) |
+        (!! sorted_tree BST && public_half g BST)
+  POST [tptr Tvoid]
+   EX ret: val,
+   PROP ()
+   LOCAL (temp ret_temp ret)
+   SEP (mem_mgr gv; nodebox_rep g sh lock b) |
+         (!! (sorted_tree BST /\ ret = lookup nullval x BST) && public_half g BST).
+
+Program Definition insert_spec :=
+  DECLARE _insert
+  ATOMIC TYPE (rmaps.ConstType (val * share * val * Z * val * globals * gname))
+  OBJ BST INVS base.empty base.top
+  WITH b:_, sh:_, lock:_, x:_, v:_, gv:_, g:_
+  PRE [_t OF (tptr (tptr t_struct_tree_t)), _x OF tint, _value OF (tptr tvoid)]
+   PROP (readable_share sh; Int.min_signed <= x <= Int.max_signed;
+       is_pointer_or_null v; is_pointer_or_null lock )
+   LOCAL (temp _t b; temp _x (Vint (Int.repr x)); temp _value v; gvars gv)
+   SEP (mem_mgr gv; nodebox_rep g sh lock b) |
+        (!! sorted_tree BST && public_half g BST)
+  POST [tvoid]
+   PROP ()
+   LOCAL ()
+   SEP (mem_mgr gv; nodebox_rep g sh lock b) |
+        (!! sorted_tree (insert x v BST) && public_half g (insert x v BST)).
+
+Definition main_spec :=
+  DECLARE _main
+          WITH gv : globals
+                      PRE  [] main_pre prog tt nil gv
+                      POST [ tint ] main_post prog nil gv.
+
+
+Definition acquire_spec := DECLARE _acquire acquire_spec.
+Definition release2_spec := DECLARE _release2 release_spec.
+Definition makelock_spec := DECLARE _makelock (makelock_spec _).
+Definition freelock2_spec := DECLARE _freelock2 (freelock2_spec _).
+
+Definition Gprog : funspecs :=
+  ltac:(with_library prog [acquire_spec; release2_spec; makelock_spec;
+                          freelock2_spec;
+                          (*
+    acquire_spec; release_spec; makelock_spec; freelock_spec;
+   makecond_spec; freecond_spec; wait_spec; signal_spec;*)
+                          surely_malloc_spec;
+                          lookup_spec; insert_spec;
+                          (* turn_left_spec; pushdown_left_spec; delete_spec ; *)
+                          (* spawn_spec; thread_func_spec; *) main_spec
+       ]).
+
+Lemma body_surely_malloc: semax_body Vprog Gprog f_surely_malloc surely_malloc_spec.
+Proof.
+  start_function.
+  forward_call (t, gv). Intros p.
+  forward_if
+  (PROP ( )
+   LOCAL (temp _p p)
+   SEP (mem_mgr gv; malloc_token Ews t p * data_at_ Ews t p)).
+  - if_tac. subst p. entailer!. entailer!.
+  - forward_call tt. contradiction.
+  - if_tac.
+    + forward. subst p. congruence.
+    + Intros. forward. entailer!.
+  - forward. Exists p; entailer!.
+Qed.
+
+Lemma tree_rep_saturate_local:
+   forall t p, tree_rep t p |-- !! is_pointer_or_null p.
+Proof. destruct t; simpl; intros. entailer!. Intros pa pb. entailer!. Qed.
+Hint Resolve tree_rep_saturate_local: saturate_local.
+
+Lemma tree_rep_valid_pointer:
+  forall t p, tree_rep t p |-- valid_pointer p.
+Proof. intros. destruct t; simpl; normalize; auto with valid_pointer. Qed.
+Hint Resolve tree_rep_valid_pointer: valid_pointer.
+
+Lemma if_trueb: forall {A: Type} b (a1 a2: A), b = true -> (if b then a1 else a2) = a1.
+Proof. intros; subst; auto. Qed.
+
+Lemma if_falseb: forall {A: Type} b (a1 a2: A), b = false -> (if b then a1 else a2) = a2.
+Proof. intros; subst; auto. Qed.
+
+Lemma node_lock_exclusive : forall g lock np,
+    exclusive_mpred (node_lock_inv g lock np).
+Proof.
+  intros. unfold node_lock_inv. unfold exclusive_mpred. unfold treebox_rep.
+  Intros tr1 tr2 tp1 tp2. sep_apply field_at_conflict; auto.
+  rewrite sepcon_comm. rewrite sepcon_FF. auto.
+Qed.
+Hint Resolve node_lock_exclusive.
+
+Lemma tree_rep_nullval: forall t, tree_rep t nullval |-- !! (t = E).
+Proof.
+  intros. destruct t; [entailer! |].
+  simpl tree_rep. Intros pa pb. entailer!.
+Qed.
+
+Hint Resolve tree_rep_nullval: saturate_local.
+
+Definition lookup_inv (b: val) (lock:val) (sh: share) (x: Z) gv (inv_names : invG)
+           (Q : val -> mpred) (g:gname) (np tp: val)
+           (root_t: tree_info) : environ -> mpred :=
+  (EX tn: val, EX t : tree_info,
+   PROP (lookup nullval x t = lookup nullval x root_t)
+   LOCAL (temp _p tn; temp _tgt np; temp _t b; temp _l lock;
+          temp _x (vint x); gvars gv)
+   SEP (data_at sh (tptr t_struct_tree_t) np b;
+       field_at sh t_struct_tree_t [StructField _lock] lock np;
+       lock_inv sh lock (node_lock_inv g lock np);
+       my_half g Tsh root_t; field_at Ews t_struct_tree_t [StructField _t] tp np;
+       malloc_token Ews t_struct_tree_t np;
+       tree_rep t tn; malloc_token Ews tlock lock;
+       tree_rep t tn -* tree_rep root_t tp;
+       atomic_shift
+         (λ BST : tree, !! sorted_tree BST && public_half g BST) ∅ ⊤
+         (λ (BST : tree) (ret : val),
+          fold_right_sepcon
+            [!! (sorted_tree BST ∧ ret = lookup nullval x BST) && public_half g BST])
+         Q; mem_mgr gv))%assert.
+
+Lemma body_lookup: semax_body Vprog Gprog f_lookup lookup_spec.
+Proof.
+  start_function.
+  unfold nodebox_rep. Intros np.
+  forward. (* _tgt = *_t; *)
+  forward. (* _l = (_tgt -> _lock); *)
+  forward_call (lock, sh, (node_lock_inv g lock np)). (* _acquire(_l); *)
+  unfold node_lock_inv at 2. unfold treebox_rep. Intros a tp.
+  change (tptr t_struct_tree) with
+      (nested_field_type t_struct_tree_t [StructField _t]).
+  rewrite <- field_at_data_at.
+  forward. (* _p = (_tgt -> _t); *)
+  forward_while (lookup_inv b lock sh x gv inv_names Q g np tp a).
+  (* while (_p != (tptr tvoid) (0)) { *)
+  - unfold lookup_inv. Exists tp a. entailer!. apply -> wand_sepcon_adjoint. cancel.
+  - entailer!.
+  - destruct t; unfold tree_rep at 1; fold tree_rep. 1: normalize. Intros pa pb.
+    forward. (* _y = (_p -> _key); *)
+    forward_if; [|forward_if].
+    + forward. Exists (pa, t1). simpl fst. simpl snd. entailer!.
+      * rewrite <- H1; simpl. rewrite if_trueb; auto. now apply Z.ltb_lt.
+      * apply RAMIF_PLAIN.trans''. apply -> wand_sepcon_adjoint. simpl.
+        Exists pa pb. entailer!.
+    + forward. Exists (pb, t2). simpl fst. simpl snd. entailer!.
+      * rewrite <- H1. simpl. rewrite if_falseb. 2: apply Z.ltb_ge; lia.
+        rewrite if_trueb; auto. now apply Z.ltb_lt.
+      * apply RAMIF_PLAIN.trans''. apply -> wand_sepcon_adjoint. simpl.
+        Exists pa pb. entailer!.
+    + assert (x = k) by lia. subst x. clear H H4 H5. forward.
+      gather_SEP (atomic_shift _ _ _ _ _) (my_half _ _ _).
+      viewshift_SEP 0 (EX y, Q y * (!! (y = v) && (my_half g Tsh a))). {
+        go_lower.
+        rewrite <- (sepcon_emp
+                      (atomic_shift (λ BST : tree_info, !! sorted_tree BST &&
+                                                        public_half g BST) ∅ ⊤
+                                    (λ (BST : tree_info) (ret : val),
+                                     !! (sorted_tree BST ∧ ret = lookup nullval k BST)
+                                     && public_half g BST * emp) Q *
+                       my_half g Tsh a)).
+        apply sync_commit_same. intro t. Intros.
+        eapply derives_trans; [|apply ghost_seplog.bupd_intro]. Exists t. cancel.
+        apply imp_andp_adjoint. Intros. rewrite if_true in H4; auto. subst t.
+        eapply derives_trans; [|apply ghost_seplog.bupd_intro].
+        rewrite <- wand_sepcon_adjoint.
+        eapply derives_trans; [|apply ghost_seplog.bupd_intro]. Exists v.
+        entailer!. rewrite <- H1. simpl.
+        now do 2 (rewrite if_falseb; [|apply Z.ltb_irrefl]). } Intros y. subst y.
+      forward_call (lock, sh, node_lock_inv g lock np).
+      * assert (Frame =
+                [Q v; mem_mgr gv; data_at sh (tptr t_struct_tree_t) np b;
+                 field_at sh t_struct_tree_t [StructField _lock] lock np]);
+          subst Frame; [ reflexivity | clear H].
+        lock_props. unfold node_lock_inv. unfold treebox_rep. Exists a tp.
+        rewrite (field_at_data_at Ews _ _ _ _). simpl nested_field_type.
+        simpl fold_right_sepcon. cancel.
+        apply modus_ponens_wand'. simpl. Exists pa pb. entailer!.
+      * forward. Exists v. unfold nodebox_rep. Exists np. entailer!.
+  - subst tn. sep_apply tree_rep_nullval. Intros. subst t. simpl in H1.
+    gather_SEP (atomic_shift _ _ _ _ _) (my_half _ _ _).
+    viewshift_SEP 0 (EX y, Q y * (!! (y = nullval) && (my_half g Tsh a))). {
+      go_lower.
+        rewrite <- (sepcon_emp
+                      (atomic_shift (λ BST : tree_info, !! sorted_tree BST &&
+                                                        public_half g BST) ∅ ⊤
+                                    (λ (BST : tree_info) (ret : val),
+                                     !! (sorted_tree BST ∧ ret = lookup nullval x BST)
+                                     && public_half g BST * emp) Q *
+                       my_half g Tsh a)).
+        apply sync_commit_same. intro tr. Intros.
+        eapply derives_trans; [|apply ghost_seplog.bupd_intro]. Exists tr. cancel.
+        apply imp_andp_adjoint. Intros. rewrite if_true in H3; auto. subst tr.
+        eapply derives_trans; [|apply ghost_seplog.bupd_intro].
+        rewrite <- wand_sepcon_adjoint.
+        eapply derives_trans; [|apply ghost_seplog.bupd_intro]. Exists nullval.
+        entailer!. } Intros y. subst y.
+    forward_call (lock, sh, node_lock_inv g lock np).
+    + assert (Frame =
+              [Q nullval; mem_mgr gv; data_at sh (tptr t_struct_tree_t) np b;
+               field_at sh t_struct_tree_t [StructField _lock] lock np]);
+        subst Frame; [ reflexivity | clear H].
+      lock_props. unfold node_lock_inv. unfold treebox_rep. Exists a tp.
+      rewrite (field_at_data_at Ews _ _ _ _). simpl nested_field_type.
+      simpl fold_right_sepcon. cancel. apply modus_ponens_wand.
+    + forward. Exists nullval. unfold nodebox_rep. Exists np. entailer!.
+Qed.
+
+Definition insert_inv (b: val) (lock:val) (sh: share) (x: Z) (v: val)
+           gv (inv_names : invG) (Q: mpred) (g:gname) (np: val)
+           (root_t: tree_info) : environ -> mpred :=
+  (EX tn: val, EX t : tree_info,
+   PROP ()
+   LOCAL (temp _tr tn; temp _tgt np; temp _t b; temp _l lock;
+          temp _x (vint x); temp _value v; gvars gv)
+   SEP (data_at sh (tptr t_struct_tree_t) np b;
+       field_at sh t_struct_tree_t [StructField _lock] lock np;
+       lock_inv sh lock (node_lock_inv g lock np);
+       my_half g Tsh root_t;
+       malloc_token Ews t_struct_tree_t np;
+       treebox_rep t tn; malloc_token Ews tlock lock;
+       treebox_rep (insert x v t) tn -* treebox_rep (insert x v root_t)
+                   (field_address t_struct_tree_t [StructField _t] np);
+       atomic_shift
+         (λ BST : verif_bst_conc_cglock2.tree, !! sorted_tree BST && public_half g BST)
+         ∅ ⊤
+         (λ (BST : verif_bst_conc_cglock2.tree) (_ : ()),
+          fold_right_sepcon
+            [!! sorted_tree (insert x v BST) && public_half g (insert x v BST)])
+         (λ _ : (), Q); mem_mgr gv))%assert.
+
+Lemma bst_left_entail: forall (t1 t1' t2: @tree val) k (v p1 p2 p b: val),
+  Int.min_signed <= k <= Int.max_signed ->
+  is_pointer_or_null v ->
+  data_at Ews (tptr t_struct_tree) p b * malloc_token Ews t_struct_tree p *
+  data_at Ews t_struct_tree (Vint (Int.repr k), (v, (p1, p2))) p *
+  tree_rep t1 p1 * tree_rep t2 p2
+  |-- treebox_rep t1 (field_address t_struct_tree [StructField _left] p) *
+       (treebox_rep t1'
+         (field_address t_struct_tree [StructField _left] p) -*
+        treebox_rep (T t1' k v t2) b).
+Proof.
+  intros.
+  unfold_data_at (data_at _ _ _ p).
+  rewrite (field_at_data_at _ t_struct_tree [StructField _left]).
+  unfold treebox_rep at 1. Exists p1. cancel.
+  rewrite <- wand_sepcon_adjoint.
+  unfold treebox_rep.
+  Exists p.
+  simpl.
+  Intros p'.
+  Exists p' p2.
+  entailer!.
+  unfold_data_at (data_at _ _ _ p).
+  rewrite (field_at_data_at _ t_struct_tree [StructField _left]).
+  cancel.
+Qed.
+
+Lemma bst_right_entail: forall (t1 t2 t2': @tree val) k (v p1 p2 p b: val),
+  Int.min_signed <= k <= Int.max_signed ->
+  is_pointer_or_null v ->
+  data_at Ews (tptr t_struct_tree) p b * malloc_token Ews t_struct_tree p *
+  data_at Ews t_struct_tree (Vint (Int.repr k), (v, (p1, p2))) p *
+  tree_rep t1 p1 * tree_rep t2 p2
+  |-- treebox_rep t2 (field_address t_struct_tree [StructField _right] p) *
+       (treebox_rep t2'
+         (field_address t_struct_tree [StructField _right] p) -*
+        treebox_rep (T t1 k v t2') b).
+Proof.
+  intros.
+  unfold_data_at (data_at _ _ _ p).
+  rewrite (field_at_data_at _ t_struct_tree [StructField _right]).
+  unfold treebox_rep at 1. Exists p2. cancel.
+  rewrite <- wand_sepcon_adjoint.
+  clear p2.
+  unfold treebox_rep.
+  Exists p.
+  simpl.
+  Intros p2.
+  Exists p1 p2.
+  entailer!.
+  unfold_data_at (data_at _ _ _ p).
+  rewrite (field_at_data_at _ t_struct_tree [StructField _right]).
+  cancel.
+Qed.
+
+Lemma body_insert: semax_body Vprog Gprog f_insert insert_spec.
+Proof.
+  start_function.
+  unfold nodebox_rep. Intros np.
+  forward. (* _tgt = *_t; *)
+  forward. (* _l = (_tgt -> _lock); *)
+  forward_call (lock, sh, (node_lock_inv g lock np)). (* _acquire(_l); *)
+  unfold node_lock_inv at 2. unfold treebox_rep. Intros tr tp.
+  forward. (* _tr = &(_tgt -> _t); *)
+  forward_loop (insert_inv b lock sh x v gv inv_names Q g np tr).
+  - unfold insert_inv. Exists (field_address t_struct_tree_t [StructField _t] np) tr.
+    entailer!. unfold treebox_rep at 1.
+    Exists tp. cancel. rewrite <- wand_sepcon_adjoint. cancel.
+  - unfold insert_inv. Intros tn t. unfold treebox_rep at 1. Intros p.
+    forward. (* _p = *_tr; *)
+    forward_if. (* if (_p == (tptr tvoid) (0)) { *)
+    + subst p.
+      forward_call (t_struct_tree, gv); [simpl; repeat (split; auto); rep_omega|].
+      Intros p'.
+      forward. (* *_tr = _p; *)
+      forward. (* (_p -> _key) = _x; *)
+      forward. (* (_p -> _value) = _value; *)
+      forward. (* (_p -> _left) = (tptr tvoid) (0); *)
+      forward. (* (_p -> _right) = (tptr tvoid) (0); *)
+      assert_PROP (t = E) by entailer!. subst t. simpl tree_rep. Intros.
+      gather_SEP (atomic_shift _ _ _ _ _) (my_half _ _ _).
+      viewshift_SEP 0 (Q * my_half g Tsh (insert x v tr)). {
+        go_lower.
+        rewrite <- (sepcon_emp
+                      (atomic_shift (λ BST : tree_info, !! sorted_tree BST &&
+                                                        public_half g BST) ∅ ⊤
+                                    (λ (BST : tree_info) (_ : ()),
+                                     !! sorted_tree (insert x v BST) &&
+                                     @public_half tree_ghost g (insert x v BST) * emp)
+                                    (λ _ : (), Q) * my_half g Tsh tr)).
+        apply sync_commit_gen1. intros tr1. Intros.
+        eapply derives_trans; [|apply ghost_seplog.bupd_intro]. Exists tr1. cancel.
+        apply imp_andp_adjoint. Intros. rewrite if_true in H3; auto. subst tr1.
+        eapply derives_trans; [|apply ghost_seplog.bupd_intro]. Exists tr tr.
+        entailer!. 2: exact tt. rewrite <- wand_sepcon_adjoint.
+        sep_apply (public_update g tr tr (insert x v tr)). Intros.
+        apply ghost_seplog.bupd_mono. entailer!. now apply insert_sorted. }
+      forward_call (lock, sh, node_lock_inv g lock np). (* _release2(_l); *)
+      * assert (Frame =
+                [Q; mem_mgr gv; data_at sh (tptr t_struct_tree_t) np b;
+                 field_at sh t_struct_tree_t [StructField _lock] lock np]);
+          subst Frame; [ reflexivity | clear H2].
+        lock_props. unfold node_lock_inv. Exists (insert x v tr).
+        simpl fold_right_sepcon. cancel. apply modus_ponens_wand'.
+        unfold treebox_rep. Exists p'. simpl. Exists nullval nullval. entailer!.
+      * forward. (* return; *) unfold nodebox_rep. Exists np. entailer!.
+    + destruct t; simpl tree_rep. 1: normalize. Intros pa pb.
+      forward. (* _y = (_p -> _key); *)
+      forward_if; [|forward_if].
+      * forward. (* _tr = &(_p -> _left); *)
+        unfold insert_inv.
+        Exists (field_address t_struct_tree [StructField _left] p) t1.
+        entailer!. simpl treebox_rep. rewrite if_trueb. 2: now apply Z.ltb_lt.
+        apply RAMIF_PLAIN.trans'. now apply bst_left_entail.
+      * forward. (* _tr = &(_p -> _right); *)
+        unfold insert_inv.
+        Exists (field_address t_struct_tree [StructField _right] p) t2.
+        entailer!. simpl treebox_rep. rewrite if_falseb. 2: apply Z.ltb_ge; lia.
+        rewrite if_trueb. 2: now apply Z.ltb_lt.
+        apply RAMIF_PLAIN.trans'. now apply bst_right_entail.
+      * assert (x = k) by lia. subst x. clear H3 H4 H5.
+        forward. (* (_p -> _value) = _value; *)
+        gather_SEP (atomic_shift _ _ _ _ _) (my_half _ _ _).
+        viewshift_SEP 0 (Q * my_half g Tsh (insert k v tr)). {
+        go_lower.
+        rewrite <- (sepcon_emp
+                      (atomic_shift (λ BST : tree_info, !! sorted_tree BST &&
+                                                        public_half g BST) ∅ ⊤
+                                    (λ (BST : tree_info) (_ : ()),
+                                     !! sorted_tree (insert k v BST) &&
+                                     @public_half tree_ghost g (insert k v BST) * emp)
+                                    (λ _ : (), Q) * my_half g Tsh tr)).
+        apply sync_commit_gen1. intros tr1. Intros.
+        eapply derives_trans; [|apply ghost_seplog.bupd_intro]. Exists tr1. cancel.
+        apply imp_andp_adjoint. Intros. rewrite if_true in H4; auto. subst tr1.
+        eapply derives_trans; [|apply ghost_seplog.bupd_intro]. Exists tr tr.
+        entailer!. 2: exact tt. rewrite <- wand_sepcon_adjoint.
+        sep_apply (public_update g tr tr (insert k v tr)). Intros.
+        apply ghost_seplog.bupd_mono. entailer!. now apply insert_sorted. }
+        forward_call (lock, sh, node_lock_inv g lock np). (* _release2(_l); *)
+        -- assert (Frame =
+                   [Q; mem_mgr gv; data_at sh (tptr t_struct_tree_t) np b;
+                    field_at sh t_struct_tree_t [StructField _lock] lock np]);
+             subst Frame; [ reflexivity | clear H3].
+           lock_props. unfold node_lock_inv. Exists (insert k v tr).
+           simpl fold_right_sepcon. cancel. apply modus_ponens_wand'.
+           unfold treebox_rep. Exists p. simpl.
+           do 2 (rewrite if_falseb; [|apply Z.ltb_irrefl]). simpl tree_rep.
+           Exists pa pb. entailer!.
+        -- forward. (* return; *) unfold nodebox_rep. Exists np. entailer!.
+Qed.
